acl2svn/branches/centaur/ld.lisp
@@ -20406,6 +20406,56 @@
 
 (deflabel note-6-2
 
+; Here is the example from Sol Swords for the item below about acl2-magic-mfc
+; and acl2-magic-canonical-pathname.  The problem was that these "placeholder"
+; functions are really clause processors, and hence should return a list of
+; clauses, not (as erroneously done before) a single clause.
+;
+;  (defun foo (x)
+;     (declare (ignore x))
+;     nil)
+;
+;  (defthm foo-of-t
+;     (foo t)
+;     :hints (("goal" :clause-processor acl2-magic-mfc)))
+;
+;  (thm nil :hints (("goal" :use foo-of-t)))
+
+; Defined function set-new-dispatch-macro-character, which we use instead of
+; set-dispatch-macro-character to extend the reader with #\@, #\!, #\u, and in
+; ACL2(h), also #\Y and #\Z.  This way, we check that the character hasn't
+; already being appropriated for the reader by the host Lisp.  Now, for
+; example, CLISP causes an error when trying to build ACL2(h), because #\Y is
+; already defined as a dispatch macro character.
+
+; Here is Robert Krug's example, trivially modified, for the heuristic
+; improvement pertaining to the ancestors check.
+
+;   (defstub rm-low-32 (addr x86) t)
+;
+;   (defaxiom n32p-rm-low-32-axiom
+;     (implies (and (integerp addr)
+;                   (<= 0 addr)
+;                   (force (< (+ 3 addr) 1000)))
+;              (and (integerp (rm-low-32 addr x86))
+;                   (<= 0 (rm-low-32 addr x86)))))
+;
+;   (defstub foo-p (x) t)
+;
+;   (defaxiom axiom-2
+;     (implies (<= 0 (rm-low-32 addr x86))
+;              (foo-p (rm-low-32 addr x86))))
+;
+;   ; The following fails, which is to be expected.  But we expect to see a forcing
+;   ; round.  This is indeed the case now, but it was not in Version 6.1 (and
+;   ; probably many versions preceding that one).
+;   (thm (implies (and (integerp addr)
+;                      (<= 0 addr))
+;                 (foo-p (rm-low-32 addr x86))))
+
+; Improved error messages and documentation pertaining to certain ill-formed
+; uses of syntaxp, in response to feedback from Robert Krug.
+
   :doc
   ":Doc-Section release-notes
 
@@ -20427,7 +20477,31 @@
 
   ~st[HEURISTIC IMPROVEMENTS]
 
+  It had been the case that an ``ancestors check'' heuristic (see source
+  function ~c[ancestors-check-builtin] if you want details) could prevent a
+  ~il[rewrite] rule's hypothesis from being rewritten to true, even when that
+  hypothesis is of the form ~c[(force <term>)].  Now, forcing will take place
+  as expected; ~pl[force].  Thanks to Robert Krug for bringing this issue to
+  our attention and sending an example, which we include as a comment in the
+  ACL2 source code (see ~c[(deflabel note-6-2 ...)]).
+
+  We further changed the ``ancestors check'' heuristic (mentioned above) so
+  that it is delayed until after we check whether the hypothesis is already
+  known, by ~il[type-set] reasoning alone (in particular, not using rewriting),
+  to be true or to be false.  We believe that this is now the ``right'' order
+  for those two operations.  We saw a slight speed up in the regression tests
+  (about a percent) with this change, but that might be in the noise.
+
   ~st[BUG FIXES]
+
+  Fixed a soundness bug that could be exploited by calling system functions
+  ~c[acl2-magic-mfc] or ~c[acl2-magic-canonical-pathname].  Thanks to Sol
+  Swords for bringing this bug to our attention.
+
+  (Windows only) On Windows, it had been possible for ACL2 not to consider two
+  pathnames to name the same file when the only difference is the case of the
+  drive, e.g., `~c[C:]' vs. `~c[c:]'.  This has been fixed.  Thanks to Sol
+  Swords for reporting this issue.
 
   ~st[CHANGES AT THE SYSTEM LEVEL]
 
@@ -25721,7 +25795,7 @@ tail recursion.
 ; have unknown constraints.
 
   (declare (xargs :guard t))
-  x)
+  (list x))
 
 #+acl2-loop-only
 (encapsulate
